No need for [eventval_valid] in [match_events]
It's only needed so that the definition of receptivity works with the
semantics of external functions, but we don't want or need receptivity
in the new approach.

As an added bonus, this means that [match_events], [match_events_query],
and [stable_event] don't need a global environment parameter any more.

common/Events.v
@@ -522,16 +522,10 @@ Inductive match_events_query: trace -> trace -> Prop :=
   | match_events_query_E0:
       match_events_query nil nil
   | match_events_query_syscall id args res1 res2:
-      eventval_valid ge res1 ->
-      eventval_valid ge res2 ->
-      eventval_type res1 = eventval_type res2 ->
       match_events_query
         (Event_syscall id args res1 :: nil)
         (Event_syscall id args res2 :: nil)
   | match_events_query_vload chunk id ofs res1 res2:
-      eventval_valid ge res1 ->
-      eventval_valid ge res2 ->
-      eventval_type res1 = eventval_type res2 ->
       match_events_query
         (Event_vload chunk id ofs res1 :: nil)
         (Event_vload chunk id ofs res2 :: nil)
@@ -544,8 +538,6 @@ Inductive match_events_query: trace -> trace -> Prop :=
         (Event_annot id args :: nil)
         (Event_annot id args :: nil)
   | match_events_query_extcall q1 q2 r1 r2:
-      extcall_valid q1 r1 ->
-      extcall_valid q2 r2 ->
       match_query cc w q1 q2 ->
       match_events_query
         (Event_extcall q1 r1 :: nil)
@@ -555,12 +547,10 @@ Inductive match_events: trace -> trace -> Prop :=
   | match_events_E0:
       match_events nil nil
   | match_events_syscall id args res:
-      eventval_valid ge res ->
       match_events
         (Event_syscall id args res :: nil)
         (Event_syscall id args res :: nil)
   | match_events_vload chunk id ofs res:
-      eventval_valid ge res ->
       match_events
         (Event_vload chunk id ofs res :: nil)
         (Event_vload chunk id ofs res :: nil)
@@ -573,8 +563,7 @@ Inductive match_events: trace -> trace -> Prop :=
         (Event_annot id args :: nil)
         (Event_annot id args :: nil)
   | match_events_extcall q1 q2 r1 r2:
-      extcall_valid q1 r1 ->
-      extcall_valid q2 r2 ->
+      (extcall_valid q1 r1 -> extcall_valid q2 r2) ->
       match_query cc w q1 q2 ->
       match_reply cc w r1 r2 ->
       match_events
@@ -592,12 +581,9 @@ Qed.
 
 Definition stable_event t :=
   match t with
-    | nil => True
-    | Event_syscall _ _ res :: nil => eventval_valid ge res
-    | Event_vload _ _ _ res :: nil => eventval_valid ge res
     | Event_extcall _ _ :: nil => False
-    | _ :: nil => True
-    | _ => False
+    | _ :: _ :: _ => False
+    | _ => True
   end.
 
 (** For stable events, we can use the simpler [match_traces] below
@@ -632,14 +618,6 @@ Proof.
   destruct 2; try contradiction; constructor; auto.
 Qed.
 
-Lemma match_events_query_match_traces t1 t2:
-  stable_event t1 ->
-  match_events_query t1 t2 ->
-  match_traces t1 t2.
-Proof.
-  destruct 2; try contradiction; constructor; auto.
-Qed.
-
 Lemma match_stable_event_refl t:
   stable_event t ->
   match_events t t.
@@ -663,13 +641,13 @@ Arguments match_events_query : clear implicits.
 
 (** Properties specific to certain calling conventions. *)
 
-Lemma match_events_id_corefl ge w t1 t2:
-  match_events ge cc_id w t1 t2 ->
+Lemma match_events_id_corefl w t1 t2:
+  match_events cc_id w t1 t2 ->
   t2 = t1.
 Proof.
   destruct 1; try congruence.
-  destruct H1.
-  inv H2.
+  destruct H0.
+  inv H1.
   simpl in *.
   congruence.
 Qed.
@@ -801,7 +779,7 @@ Record extcall_properties (sem: extcall_sem) (sg: signature) : Prop :=
     sem ge vargs m1 t vres m2 ->
     Mem.extends m1 m1' ->
     Val.lessdef_list vargs vargs' ->
-    exists w, forall t', match_events ge cc_extends w t t' ->
+    exists w, forall t', match_events cc_extends w t t' ->
     exists vres', exists m2',
        sem ge vargs' m1' t' vres' m2'
     /\ Val.lessdef vres vres'
@@ -816,7 +794,7 @@ Record extcall_properties (sem: extcall_sem) (sg: signature) : Prop :=
     sem ge1 vargs m1 t vres m2 ->
     Mem.inject f m1 m1' ->
     Val.inject_list f vargs vargs' ->
-    exists w, forall t', match_events ge2 cc_inject w t t' ->
+    exists w, forall t', match_events cc_inject w t t' ->
     exists f', exists vres', exists m2',
        sem ge2 vargs' m1' t' vres' m2'
     /\ Val.inject f' vres vres'
@@ -844,10 +822,10 @@ Record extcall_properties (sem: extcall_sem) (sg: signature) : Prop :=
     match_traces ge t1 t2 /\ (t1 = t2 -> vres1 = vres2 /\ m1 = m2)
 }.
 
-Lemma stable_step cc ge t (P: world cc -> trace -> Prop):
-  stable_event ge t ->
+Lemma stable_step cc t (P: world cc -> trace -> Prop):
+  stable_event t ->
   P dummy_world t ->
-  exists w, forall t', match_events ge cc w t t' -> P w t'.
+  exists w, forall t', match_events cc w t t' -> P w t'.
 Proof.
   intros Ht H.
   exists dummy_world.
@@ -944,8 +922,7 @@ Proof.
 - inv H. inv H1. inv H6. inv H4.
   apply stable_step.
   {
-    destruct H2; try constructor.
-    inv H2; simpl; eauto.
+    destruct H2; constructor.
   }
   exploit volatile_load_extends; eauto. intros [v' [A B]].
   exists v'; exists m1'; intuition. constructor; auto.
@@ -953,9 +930,7 @@ Proof.
 - inv H0. inv H2. inv H7. inversion H5; subst.
   apply stable_step.
   {
-    destruct H3; try constructor.
-    destruct H as [? _].
-    inv H3; simpl; eauto.
+    destruct H3; constructor.
   }
   exploit volatile_load_inject; eauto. intros [v' [A B]].
   exists f; exists v'; exists m1'; intuition. constructor; auto.
@@ -1594,7 +1569,7 @@ Proof.
     inv Ht'.
     assert (q2 = cq id sg vargs' m1') by eauto using match_query_determ; subst.
     destruct r2 as [vres' m2'].
-    specialize (Hr _ _ _ _ H8).
+    specialize (Hr _ _ _ _ H7).
     exists vres', m2'; intuition.
     constructor.
     assumption.
@@ -1718,7 +1693,7 @@ Lemma external_call_mem_inject:
   external_call ef ge vargs m1 t vres m2 ->
   Mem.inject f m1 m1' ->
   Val.inject_list f vargs vargs' ->
-  exists w, forall t', match_events ge cc_inject w t t' ->
+  exists w, forall t', match_events cc_inject w t t' ->
   exists f', exists vres', exists m2',
      external_call ef ge vargs' m1' t' vres' m2'
     /\ Val.inject f' vres vres'
