backend/Deadcodeproof.v
@@ -732,7 +732,7 @@ Qed.
 Theorem step_simulation:
   forall S1 t S2, step ge S1 t S2 ->
   forall S1', match_states S1 S1' -> sound_state prog S1 ->
-  exists w, forall t', match_events ge cc_extends w t t' ->
+  exists w, forall t', match_events cc_extends w t t' ->
   exists S2', step tge S1' t' S2' /\ match_states S2 S2'.
 Proof.
 
