backend/Inliningproof.v
@@ -1023,7 +1023,7 @@ Theorem step_simulation:
   forall S1 t S2,
   step ge S1 t S2 ->
   forall S1' (MS: match_states S1 S1'),
-  exists w, forall t', match_events ge cc_inject w t t' ->
+  exists w, forall t', match_events cc_inject w t t' ->
   (exists S2', plus step tge S1' t' S2' /\ match_states S2 S2')
   \/ (measure S2 < measure S1 /\ t = E0 /\ match_states S2 S1')%nat.
 Proof.
