cfrontend/SimplLocalsproof.v
@@ -2002,7 +2002,7 @@ End FIND_LABEL.
 Lemma step_simulation:
   forall S1 t S2, step1 ge S1 t S2 ->
   forall S1' (MS: match_states S1 S1'),
-  exists w, forall t', match_events ge cc_inject w t t' ->
+  exists w, forall t', match_events cc_inject w t t' ->
   exists S2', plus step2 tge S1' t' S2' /\ match_states S2 S2'.
 Proof.
   induction 1; simpl; intros; inv MS; simpl in *; try (monadInv TRS); try stable_step.
